RelationalAlgebra/Equivalence/Equivalence.lean
@@ -3,10 +3,10 @@ import RelationalAlgebra.Equivalence.RAtoFOL.Selection
 import RelationalAlgebra.Equivalence.RAtoFOL.Projection
 import RelationalAlgebra.Equivalence.RAtoFOL.Join
 import RelationalAlgebra.Equivalence.RAtoFOL.Rename
+import RelationalAlgebra.Equivalence.RAtoFOL.Union
+import RelationalAlgebra.Equivalence.RAtoFOL.Diff
 
 open RM
-
-set_option maxHeartbeats 2000000
 
 theorem ra_to_fol_evalT {raQ dbi} [struc : FOL.folStruc dbi] (h : RA.Query.isWellTyped dbi.schema raQ) :
   (ra_to_fol_query raQ dbi.schema).evaluateT dbi = RA.Query.evaluateT dbi raQ := by
@@ -16,55 +16,8 @@ theorem ra_to_fol_evalT {raQ dbi} [struc : FOL.folStruc dbi] (h : RA.Query.isWel
     | p rs sq ih => exact ra_to_fol_evalT.p_def_eq h (ih h.1)
     | j q₁ q₂ ih₁ ih₂ => exact ra_to_fol_evalT.j_def_eq h (ih₁ h.1) (ih₂ h.2)
     | r f q ih => exact ra_to_fol_evalT.r_def_eq h (ih h.1)
-    | u q₁ q₂ ih₁ ih₂ =>
-      simp_all [ra_to_fol_query, ra_to_fol_query_schema]
-      simp [FOL.Query.evaluateT, FOL.BoundedQuery.Realize, unionT, ← ih₁, ← ih₂]
-      simp_all [ra_to_fol_query_schema]
-      ext t
-      unfold FOL.TupleToFun
-      simp_all only [Set.mem_setOf_eq, Set.mem_union]
-      obtain ⟨left, right⟩ := h
-      obtain ⟨left_1, right⟩ := right
-      apply Iff.intro
-      · intro a
-        simp_all only [forall_true_left, true_and]
-        obtain ⟨left_2, right_1⟩ := a
-        convert right_1 left_2
-      · intro a
-        cases a with
-        | inl h =>
-          simp_all only [forall_true_left, true_and]
-          obtain ⟨left_2, right_1⟩ := h
-          apply Or.inl
-          convert right_1 left_2
-        | inr h_1 =>
-          simp_all only [forall_true_left, true_and]
-          obtain ⟨left_2, right_1⟩ := h_1
-          apply Or.inr
-          convert right_1 left_2
-    | d q nq ih nih =>
-      simp_all [ra_to_fol_query, ra_to_fol_query_schema]
-      simp [FOL.Query.evaluateT, FOL.BoundedQuery.Realize, diffT, ← ih, ← nih, Set.diff]
-      simp_all [ra_to_fol_query_schema]
-      ext t
-      unfold FOL.TupleToFun
-      simp_all only [Set.mem_setOf_eq]
-      obtain ⟨left, right⟩ := h
-      obtain ⟨left_1, right⟩ := right
-      apply Iff.intro
-      . intro h
-        apply And.intro
-        . apply And.intro h.1
-          intro x
-          convert (h.2 x).1
-        . intro x
-          convert (h.2 x).2
-      . intro h
-        apply And.intro h.1.1
-        intro x
-        apply And.intro
-        . convert h.1.2 x
-        . convert h.2 x
+    | u q₁ q₂ ih₁ ih₂ => exact ra_to_fol_evalT.u_def_eq h (ih₁ h.1) (ih₂ h.2.1)
+    | d q nq ih nih => exact ra_to_fol_evalT.d_def_eq h (ih h.1) (nih h.2.1)
 
 theorem ra_to_fol_eval {dbi} [struc : FOL.folStruc dbi] (raQ : RA.Query) (h_ra_wt : raQ.isWellTyped dbi.schema) :
   (ra_to_fol_query raQ dbi.schema).evaluate dbi = raQ.evaluate dbi h_ra_wt := by
