RelationalAlgebra/Equivalence/RAtoFOL/Join.lean
@@ -14,7 +14,7 @@ theorem ra_to_fol_evalT.j_def.mp (h : RA.Query.isWellTyped dbi.schema (.j q₁ q
         Set.mem_setOf_eq] at ⊢ h
       simp only [FOL.BoundedQuery.Realize, FOL.BoundedQuery.toFormula_and,
         FirstOrder.Language.BoundedFormula.realize_inf, and_imp]
-      intro a_2 a_3
+      intro a_2 a_3 a_4
       have h_dom : t.Dom = ↑(q₁.schema dbi.schema) ∪ ↑(q₂.schema dbi.schema) := by
         rw [← ra_to_fol_query_schema h.1, ← ra_to_fol_query_schema h.2]; simp_all
 
@@ -23,38 +23,32 @@ theorem ra_to_fol_evalT.j_def.mp (h : RA.Query.isWellTyped dbi.schema (.j q₁ q
       apply And.intro
       . apply ih₁
         . simp_all only [FOL.Query.RealizeMin, Pi.default_def, Nat.default_eq_zero, and_imp, forall_true_left]
-          simp_all only
           obtain ⟨left, right⟩ := h
-          obtain ⟨left_1, right_1⟩ := a_3
-          apply And.intro
-          · rfl
-          · intro h
-            rw [FOL.BoundedQuery.Realize.enlarge]
-            exact left_1
+          apply Exists.intro
+          · rw [FOL.BoundedQuery.Realize.enlarge]
+            exact a_3
             . simp [Set.subset_def, PFun.mem_dom]
             . rfl
             . rfl
             . rfl
             . simp_all only [FOL.BoundedQuery.schema.and_def, Finset.coe_union]
+          · rfl
 
       . have z' : ↑(ra_to_fol_query q₂ dbi.schema).schema ⊆ t.Dom := by simp_all [ra_to_fol_query_schema]
         use t.restrict z'
         apply And.intro
         . apply ih₂
           . simp_all only [FOL.Query.RealizeMin, Pi.default_def, Nat.default_eq_zero, and_imp, forall_true_left]
-            simp_all only
             obtain ⟨left, right⟩ := h
-            obtain ⟨left_1, right_1⟩ := a_3
-            apply And.intro
-            · rfl
-            · intro h
-              rw [FOL.BoundedQuery.Realize.enlarge]
-              exact right_1
+            apply Exists.intro
+            · rw [FOL.BoundedQuery.Realize.enlarge]
+              exact a_4
               . simp [Set.subset_def, PFun.mem_dom]
               . rfl
               . rfl
               . rfl
               . simp_all only [FOL.BoundedQuery.schema.and_def, Finset.coe_union]
+            · rfl
 
         . intro a
           simp only [PFun.mem_restrict, Finset.mem_coe, and_imp, not_and]
@@ -95,7 +89,7 @@ theorem ra_to_fol_evalT.j_def.mpr (h : RA.Query.isWellTyped dbi.schema (.j q₁ 
       have t_Dom : t.Dom = q₁.schema dbi.schema ∪ q₂.schema dbi.schema := by
         exact RA.Query.evaluate.validSchema (.j q₁ q₂) h t h_RA_eval
 
-      apply And.intro (by simp_all [ra_to_fol_query_schema])
+      apply Exists.intro (by simp_all [ra_to_fol_query_schema])
 
       simp only [ra_to_fol_query]
       simp_all only [RA.Query.isWellTyped.j_def, RA.Query.evaluateT.j_def, joinT, PFun.mem_dom,
@@ -110,7 +104,6 @@ theorem ra_to_fol_evalT.j_def.mpr (h : RA.Query.isWellTyped dbi.schema (.j q₁ 
       obtain ⟨hw₂, right_1⟩ := h
       simp only [FOL.BoundedQuery.Realize, FOL.BoundedQuery.toFormula_and,
         FirstOrder.Language.BoundedFormula.realize_inf]
-      intro h'
       apply And.intro
       · have w_Dom : w₁.Dom = q₁.schema dbi.schema := by
           exact RA.Query.evaluate.validSchema q₁ left w₁ hw₁
@@ -118,8 +111,8 @@ theorem ra_to_fol_evalT.j_def.mpr (h : RA.Query.isWellTyped dbi.schema (.j q₁ 
         simp_all only [Finset.coe_union, and_self, Set.subset_union_left, FOL.BoundedQuery.Realize]
         have z := (ih₁ w₁ hw₁)
         have ⟨h_sub, ht'⟩ : ∃h_sub : w₁.Dom ⊆ t.Dom, t.restrict h_sub = w₁ := by
-          simp_all only [FOL.BoundedQuery.schema.and_def, Finset.coe_union, Pi.default_def,
-            Nat.default_eq_zero, imp_self, and_self, exists_true_left]
+          simp_all only [Finset.coe_union, Pi.default_def, Nat.default_eq_zero, Finset.coe_inj,
+            Set.subset_union_left, exists_true_left]
           ext a v; simp [*]
           simp_all only [FOL.BoundedQuery.schema.and_def, Finset.coe_union, Pi.default_def, Nat.default_eq_zero,
             imp_self, and_self, implies_true]
@@ -138,8 +131,8 @@ theorem ra_to_fol_evalT.j_def.mpr (h : RA.Query.isWellTyped dbi.schema (.j q₁ 
             · simp_all [(right_1 a).1 v a_1]
 
         rw [← FOL.BoundedQuery.Realize]
-        rw [← FOL.BoundedQuery.Realize.enlarge h_sub ht' (by simp_all [ra_to_fol_query_schema])]
-        . exact (z.2 z.1)
+        rw [← FOL.BoundedQuery.Realize.enlarge h_sub ht' (by simp [ra_to_fol_query_schema left, w_Dom])]
+        . exact z.2
         . simp [ra_to_fol_query_schema left, z.1]
         . simp [t_Dom, ra_to_fol_query_schema left, ra_to_fol_query_schema right]
 
@@ -169,8 +162,8 @@ theorem ra_to_fol_evalT.j_def.mpr (h : RA.Query.isWellTyped dbi.schema (.j q₁ 
             · simp_all [(right_1 a).2.1 v a_1]
 
         rw [← FOL.BoundedQuery.Realize]
-        rw [← FOL.BoundedQuery.Realize.enlarge h_sub ht' (by simp_all [ra_to_fol_query_schema])]
-        . exact (z.2 z.1)
+        rw [← FOL.BoundedQuery.Realize.enlarge h_sub ht' (by simp [ra_to_fol_query_schema right, w_Dom])]
+        . exact z.2
         . simp [ra_to_fol_query_schema right, z.1]
         . simp [t_Dom, ra_to_fol_query_schema left, ra_to_fol_query_schema right]
 
