RelationalAlgebra/Equivalence/RAtoFOL/Selection.lean
@@ -7,14 +7,13 @@ theorem ra_to_fol_evalT.s_def.mp (h : RA.Query.isWellTyped dbi.schema (.s a b q)
     ∀t, (ra_to_fol_query (.s a b q) dbi.schema).RealizeMin dbi t → t ∈ RA.Query.evaluateT dbi (.s a b q) := by
       intro t
       simp [RA.Query.isWellTyped.s_def, ra_to_fol_query, FOL.outVar.def,
-        FOL.Query.RealizeMin, FOL.BoundedQuery.Realize, FOL.BoundedQuery.toFormula_and,
+        FOL.Query.RealizeMin.ex_def, FOL.BoundedQuery.Realize, FOL.BoundedQuery.toFormula_and,
         FOL.BoundedQuery.toFormula_tEq, FirstOrder.Language.BoundedFormula.realize_inf,
         FOL.BoundedQuery.schema.and_def, FOL.BoundedQuery.schema.tEq_def,
         FirstOrder.Language.Term.varFinsetLeft, Finset.coe_union, Finset.coe_singleton,
         Set.union_singleton, Set.union_insert, RA.Query.evaluateT.s_def, selectionT,
         Set.mem_setOf_eq, and_imp] at ⊢ h
-      intro a_1 a_2
-      simp_all [FOL.BoundedQuery.Realize, and_imp]
+      intro a_1 a_2 a_3
       obtain ⟨left, right⟩ := h
       obtain ⟨left_1, right⟩ := right
       simp [ra_to_fol_query_schema, left, left_1, right] at ih a_1
@@ -22,41 +21,38 @@ theorem ra_to_fol_evalT.s_def.mp (h : RA.Query.isWellTyped dbi.schema (.s a b q)
       simp [FOL.TupleToFun.def _] at *
       apply And.intro
       · apply ih
-        . simp_all
-        · exact a_1
-      · obtain ⟨l, r⟩ := a_2
-        simp [FirstOrder.Language.BoundedFormula.Realize] at r
+        simp [FOL.Query.RealizeMin.ex_def]
+        apply And.intro
+        · simp [ra_to_fol_query_schema left, a_1]
+        · exact a_2
+      · simp [FirstOrder.Language.BoundedFormula.Realize] at a_3
         have : (t a).Dom := by simp_all [Part.dom_iff_mem, ← PFun.mem_dom]
         have : (t b).Dom := by simp_all [Part.dom_iff_mem, ← PFun.mem_dom]
-        simp [Part.getOrElse, *] at r
+        simp [Part.getOrElse, *] at a_3
         simp_all [Part.ext_iff, Part.mem_eq]
 
 theorem ra_to_fol_evalT.s_def.mpr (h : RA.Query.isWellTyped dbi.schema (.s a b q))
   (ih : ∀t ∈ RA.Query.evaluateT dbi q, (ra_to_fol_query q dbi.schema).RealizeMin dbi t) :
     ∀t, t ∈ RA.Query.evaluateT dbi (.s a b q) → (ra_to_fol_query (.s a b q) dbi.schema).RealizeMin dbi t := by
       intro t h_RA_eval
-      apply And.intro
-        (by simp_all [RA.Query.evaluate.validSchema (.s a b q) h t h_RA_eval, ra_to_fol_query_schema])
+      have h_1 := RA.Query.evaluate.validSchema (.s a b q) h t h_RA_eval
+      apply Exists.intro
+        (by simp_all [h_1, ra_to_fol_query_schema])
 
-      simp only [ra_to_fol_query]
-      intro h_1
-      simp [FOL.BoundedQuery.schema] at h_1
-      rw [← FOL.BoundedQuery.schema] at h_1
-      simp_all only [RA.Query.isWellTyped.s_def, FOL.Query.RealizeMin, Pi.default_def, Nat.default_eq_zero,
+      unfold FOL.TupleToFun
+      simp only [ra_to_fol_query, FOL.BoundedQuery.Realize]
+      simp_all only [RA.Query.isWellTyped.s_def, FOL.Query.RealizeMin.ex_def, Pi.default_def, Nat.default_eq_zero,
         RA.Query.evaluateT.s_def, FOL.outVar.def]
       obtain ⟨left, right⟩ := h
       obtain ⟨left_1, right⟩ := right
       simp_all [FOL.BoundedQuery.Realize, selectionT]
       simp [ra_to_fol_query_schema, left, left_1, right] at *
       have dec_a := FOL.dec_dom h_1
-      simp [FOL.TupleToFun.def _] at *
-      simp_all only [FOL.outVar.def, FOL.BoundedQuery.schema.and_def, FOL.BoundedQuery.schema.tEq_def,
-        FirstOrder.Language.Term.varFinsetLeft, Finset.coe_union, Finset.coe_singleton, Set.union_singleton,
-        Set.union_insert]
       apply And.intro
-      · have := (ih t h_RA_eval.1).2 (by simp_all)
+      · have := (ih t h_RA_eval.1).2
         simp_all only [and_self, imp_self, implies_true, FOL.TupleToFun.def, Nat.default_eq_zero]
-      · simp [FirstOrder.Language.BoundedFormula.Realize, h_RA_eval.2]
+        convert this
+      · simp [FirstOrder.Language.BoundedFormula.Realize, h_RA_eval.2]; convert rfl
 
 theorem ra_to_fol_evalT.s_def_eq (h : RA.Query.isWellTyped dbi.schema (.s a b q))
   (ih: (ra_to_fol_query q dbi.schema).evaluateT dbi = RA.Query.evaluateT dbi q) :
