RelationalAlgebra/Equivalence/RAtoFOL/Union.lean
@@ -1,0 +1,33 @@
+import RelationalAlgebra.Equivalence.RAtoFOL.Conversion
+
+variable {dbi q₁ q₂} [FOL.folStruc dbi]
+
+theorem ra_to_fol_evalT.u_def_eq (h : RA.Query.isWellTyped dbi.schema (.u q₁ q₂))
+  (ih₁ : FOL.Query.evaluateT dbi (ra_to_fol_query q₁ dbi.schema) = RA.Query.evaluateT dbi q₁)
+  (ih₂ : FOL.Query.evaluateT dbi (ra_to_fol_query q₂ dbi.schema) = RA.Query.evaluateT dbi q₂) :
+    FOL.Query.evaluateT dbi (ra_to_fol_query (q₁.u q₂) dbi.schema) = RA.Query.evaluateT dbi (q₁.u q₂) := by
+      simp_all [ra_to_fol_query, ra_to_fol_query_schema]
+      simp [FOL.Query.evaluateT, FOL.Query.RealizeMin.and_def, FOL.BoundedQuery.Realize, unionT, ← ih₁, ← ih₂]
+      simp_all [ra_to_fol_query_schema]
+      ext t
+      unfold FOL.TupleToFun
+      simp_all only [Set.mem_setOf_eq, Set.mem_union]
+      obtain ⟨left, right⟩ := h
+      obtain ⟨left_1, right⟩ := right
+      apply Iff.intro
+      · intro a
+        simp_all only [forall_true_left, true_and]
+        obtain ⟨left_2, right_1⟩ := a
+        convert right_1 left_2
+      · intro a
+        cases a with
+        | inl h =>
+          simp_all only [forall_true_left, true_and]
+          obtain ⟨left_2, right_1⟩ := h
+          apply Or.inl
+          convert right_1 left_2
+        | inr h_1 =>
+          simp_all only [forall_true_left, true_and]
+          obtain ⟨left_2, right_1⟩ := h_1
+          apply Or.inr
+          convert right_1 left_2
